doc/simple/coq/Subst.v
@@ -4,6 +4,8 @@ Require Import AlgoDef.
 Require Import UtilityEnv.
 Require Import DeclDef.
 
+Set Implicit Arguments.
+
 Lemma ctxsubst_inv_empty : forall I,
     ACpltCtxSubstCtx empty empty I ->
     I = empty.
@@ -59,19 +61,206 @@ Proof.
   destruct (eq_push_inv H2) as [? [? ?]]. false.
 Qed.
 
+Lemma ctxsubst_inv_bndvar : forall H G I' x s1 s2 t1 t2,
+    ACpltCtxSubstCtx (H & x ~ AC_Bnd s1 t1) (G & x ~ AC_Bnd s2 t2) I' ->
+    exists I s1' t1', (I' = I & x ~ DC_Bnd s1' t1' /\
+      CompleteCtx H /\ ACpltCtxSubstCtx H G I /\
+      ACtxSubst H t1 = ACtxSubst H t2 /\
+      ACtxTSubst H s1 = ACtxTSubst H s2 /\
+      ACpltCtxSubst H t1 t1' /\
+      ACpltCtxTSubst H s1 s1').
+Proof.
+  intros. inversions H0.
+  false. apply* empty_push_inv.
+  destruct (eq_push_inv H2) as [? [? ?]]. false.
+  destruct (eq_push_inv H2) as [? [? ?]]. false.
+  exists I s1' t1'.
+  destruct (eq_push_inv H2) as [? [? ?]]; subst.
+  destruct (eq_push_inv H3) as [? [? ?]]; subst.
+  inversions H10; inversions H1.
+  split*.
+  destruct (eq_push_inv H2) as [? [? ?]]. false.
+  destruct (eq_push_inv H2) as [? [? ?]]. false.
+  destruct (eq_push_inv H2) as [? [? ?]]. false.
+Qed.
+
+Lemma ctxsubst_inv_suevar : forall H G I a t,
+    ACpltCtxSubstCtx (H & a ~ AC_Solved_EVar t) (G & a ~ AC_Unsolved_EVar) I ->
+    CompleteCtx H /\
+    ACpltCtxSubstCtx H G I.
+Proof.
+  intros. inversions H0.
+  false. apply* empty_push_inv.
+  destruct (eq_push_inv H2) as [? [? ?]]. false.
+  destruct (eq_push_inv H2) as [? [? ?]].
+  false.
+  destruct (eq_push_inv H2) as [? [? ?]].
+  false.
+  destruct (eq_push_inv H2) as [? [? ?]]; subst.
+  destruct (eq_push_inv H3) as [? [? ?]]; subst.
+  auto.
+  destruct (eq_push_inv H3) as [? [? ?]].
+  false.
+  destruct (eq_push_inv H2) as [? [? ?]]; subst.
+  auto.
+  false.
+  assert (binds a AC_Unsolved_EVar (G & a ~ AC_Unsolved_EVar)).
+  apply* binds_tail.
+  apply binds_fresh_inv with (A := ACtxT) (x := a) (v := AC_Unsolved_EVar) (E := G & a ~ AC_Unsolved_EVar).
+  auto. auto.
+Qed.
+
+Lemma ctxsubst_inv_ssevar : forall H G I t1 t2 a,
+    ACpltCtxSubstCtx (H & a ~ AC_Solved_EVar t1) (G & a ~ AC_Solved_EVar t2) I ->
+    CompleteCtx H /\
+    ACpltCtxSubstCtx H G I /\
+    ACtxSubst H t1 = ACtxSubst H t2.
+Proof.
+  intros. inversions H0.
+  false. apply* empty_push_inv.
+  destruct (eq_push_inv H2) as [? [? ?]]. false.
+  destruct (eq_push_inv H2) as [? [? ?]].
+  false.
+  destruct (eq_push_inv H2) as [? [? ?]].
+  false.
+  destruct (eq_push_inv H3) as [? [? ?]]; false.
+  destruct (eq_push_inv H2) as [? [? ?]]; subst.
+  destruct (eq_push_inv H3) as [? [? ?]]; subst.
+  inversions H1; inversions H7.
+  auto.
+  destruct (eq_push_inv H2) as [? [? ?]]; subst.
+  auto.
+  false.
+  assert (binds a AC_Unsolved_EVar (G & a ~ AC_Unsolved_EVar)).
+  apply* binds_tail.
+  apply binds_fresh_inv with (A := ACtxT) (x := a) (v := AC_Unsolved_EVar) (E := G & a ~ AC_Unsolved_EVar).
+  auto. auto.
+Qed.
+
+Lemma ctxsubst_inv_sevar : forall H G I t a,
+    ACpltCtxSubstCtx (H & a ~ AC_Solved_EVar t) G I ->
+    a # G ->
+    CompleteCtx H /\
+    ACpltCtxSubstCtx H G I.
+Proof.
+  intros. inversions H0.
+  false. apply* empty_push_inv.
+  destruct (eq_push_inv H3) as [? [? ?]]. false.
+  destruct (eq_push_inv H3) as [? [? ?]]. false.
+  destruct (eq_push_inv H3) as [? [? ?]]. false.
+  
+  destruct (eq_push_inv H3) as [? [? ?]]; subst.
+  assert (binds a AC_Unsolved_EVar (G0 & a ~ AC_Unsolved_EVar)).
+  apply* binds_tail.
+  false.
+  apply binds_fresh_inv with (A := ACtxT) (x := a) (v := AC_Unsolved_EVar) (E := G0 & a ~ AC_Unsolved_EVar).
+  auto. auto.
+
+  destruct (eq_push_inv H3) as [? [? ?]]; subst.
+  assert (binds a AC_Unsolved_EVar (G0 & a ~ AC_Unsolved_EVar)).
+  apply* binds_tail.
+  false.
+  apply binds_fresh_inv with (A := ACtxT) (x := a) (v := AC_Unsolved_EVar) (E := G0 & a ~ AC_Unsolved_EVar).
+  auto. auto.
+
+  destruct (eq_push_inv H3) as [? [? ?]]; subst.
+  auto.
+Qed.
+
+Lemma ctxsubst_inv_uuevar : forall H G I a,
+    ACpltCtxSubstCtx (H & a ~ AC_Unsolved_EVar) (G & a ~ AC_Unsolved_EVar) I -> False.
+Proof.
+  intros. inversions H0.
+  false. apply* empty_push_inv.
+  destruct (eq_push_inv H2) as [? [? ?]]. false.
+  destruct (eq_push_inv H2) as [? [? ?]]. false.
+  destruct (eq_push_inv H2) as [? [? ?]]. false.
+  destruct (eq_push_inv H2) as [? [? ?]]. false.
+  destruct (eq_push_inv H2) as [? [? ?]]. false.
+  destruct (eq_push_inv H2) as [? [? ?]]. false.
+Qed.
+
+Lemma cplt_ctxsubst_eq : forall G t1 t2 t2',
+    ACpltCtxSubst G t1 t2 ->
+    ACpltCtxSubst G t1 t2' ->
+    t2 = t2'.
+Proof.
+  introv Hyp1. gen t2'. inductions Hyp1; introv Hyp2; inversions Hyp2; auto.
+  (* FIXME!!! *)
+  admit. 
+  rewrite -> (IHHyp1_1 d0 H2).
+  rewrite -> (IHHyp1_2 d3 H4).
+  auto.
+  rewrite -> (IHHyp1 d0 H1).
+  auto.
+  rewrite -> (IHHyp1_1 d0 H2).
+  rewrite -> (IHHyp1_2 d3 H4).
+  auto.
+  rewrite -> (IHHyp1_1 d0 H2).
+  rewrite -> (IHHyp1_2 d3 H4).
+  auto.
+  rewrite -> (IHHyp1 d0 H1).
+  auto.
+  rewrite -> (IHHyp1 d0 H1).
+  auto.
+  rewrite -> (IHHyp1_1 d0 H2).
+  rewrite -> (IHHyp1_2 d3 H4).
+  auto.
+Qed.
+
+Lemma cplt_ctxtsubst_eq : forall G t1 t2 t2',
+    ACpltCtxTSubst G t1 t2 ->
+    ACpltCtxTSubst G t1 t2' ->
+    t2 = t2'.
+Proof.
+  introv Hyp1. gen t2'. inductions Hyp1; introv Hyp2; inversions Hyp2; auto.
+  pose (IHHyp1 s3 H1).
+  rewrite* e.
+  assert (t2 = t3).
+  apply* cplt_ctxsubst_eq.
+  rewrite* H0.
+Qed.
+
 Lemma stable_cplt_env : forall G H I J,
     ExtCtx G H ->
     ACpltCtxSubstCtx H G I ->
     ACpltCtxSubstCtx H H J ->
     I = J.
 Proof.
-  intros. inductions H0.
-  pose (ctxsubst_inv_empty I H1).
-  pose (ctxsubst_inv_empty J H2).
+  intros. gen I J. inductions H0; intros.
+  pose (ctxsubst_inv_empty H1).
+  pose (ctxsubst_inv_empty H2).
   rewrite e. rewrite e0. auto.
-  destruct (ctxsubst_inv_var H G I x H3) as [_ ?].
-  destruct (ctxsubst_inv_var H H J x H4) as [_ ?].
+  destruct (ctxsubst_inv_var H3) as [_ ?].
+  destruct (ctxsubst_inv_var H4) as [_ ?].
   apply* IHExtCtx.
-  destruct (ctxsubst_inv_typvar H G I x t2 t1 H4) as [I1' [t1' [? [_ [? ?]]]]].
-Admitted.
-  
+  destruct (ctxsubst_inv_typvar H4) as [I1' [t1' [? [? [? [? ?]]]]]].
+  destruct (ctxsubst_inv_typvar H5) as [I2' [t2' [? [? [? [? ?]]]]]].
+  pose (cplt_ctxsubst_eq H10 H15).
+  pose (IHExtCtx I1' H8 I2' H13).
+  rewrite H6.
+  rewrite H11.
+  rewrite e.
+  rewrite e0.
+  auto.
+  destruct (ctxsubst_inv_bndvar H5) as [I1' [s1' [t1' [? [? [? [? [? [? ?]]]]]]]]].
+  destruct (ctxsubst_inv_bndvar H6) as [I2' [s2' [t2' [? [? [? [? [? [? ?]]]]]]]]].
+  pose (IHExtCtx I1' H9 I2' H16).
+  pose (cplt_ctxsubst_eq H12 H19).
+  pose (cplt_ctxtsubst_eq H13 H20).
+  rewrite H7. rewrite H14. rewrite e; rewrite e0; rewrite e1. auto.
+  false. pose (ctxsubst_inv_uuevar H3). auto.
+  destruct (ctxsubst_inv_ssevar H4) as [? [? ?]].
+  destruct (ctxsubst_inv_ssevar H5) as [? [? ?]].
+  apply* IHExtCtx.
+  destruct (ctxsubst_inv_suevar H3) as [? ?].
+  destruct (ctxsubst_inv_ssevar H4) as [? [? ?]].
+  apply* IHExtCtx.
+  false. pose (ctxsubst_inv_uuevar H3). auto.
+  (* FIXME!!! *)
+  assert (a # G). admit.
+  destruct (ctxsubst_inv_sevar H2 H4) as [? ?].
+  destruct (ctxsubst_inv_ssevar H3) as [? [? ?]].
+  apply* IHExtCtx.
+Qed.
+
